correctness/RegexCorrectness/Strategy/Materialize/Basic.lean
@@ -3,7 +3,7 @@ import RegexCorrectness.Data.Expr.Semantics.CaptureGroups
 set_option autoImplicit false
 
 open Regex.Data (CaptureGroups)
-open String (ValidPos ValidPosPlusOne)
+open String (Pos ValidPosPlusOne)
 
 namespace Regex.Strategy
 
@@ -13,7 +13,7 @@ variable {s : String}
 `materializeRegexGroups groups` constructs a mapping that associates each capture group's tag
 with the start/end positions of the last appearance of the capture group in the input string.
 -/
-def materializeRegexGroups : CaptureGroups s → Nat → Option (ValidPos s × ValidPos s)
+def materializeRegexGroups : CaptureGroups s → Nat → Option (Pos s × Pos s)
   | .empty, _ => .none
   | .group tag first last groups, tag' =>
     if tag = tag' then
@@ -24,7 +24,7 @@ def materializeRegexGroups : CaptureGroups s → Nat → Option (ValidPos s × V
     -- The later one will be preferred
     materializeRegexGroups g₂ tag <|> materializeRegexGroups g₁ tag
 
-def materializeUpdatesAux (n : Nat) (accum : Vector (ValidPosPlusOne s) n) : List (Nat × ValidPos s) → Vector (ValidPosPlusOne s) n
+def materializeUpdatesAux (n : Nat) (accum : Vector (ValidPosPlusOne s) n) : List (Nat × Pos s) → Vector (ValidPosPlusOne s) n
   | [] => accum
   | (offset, pos) :: rest =>
     materializeUpdatesAux n (accum.setIfInBounds offset (.validPos pos)) rest
@@ -34,16 +34,16 @@ def materializeUpdatesAux (n : Nat) (accum : Vector (ValidPosPlusOne s) n) : Lis
 as the writes to the buffer. When the same offset appears multiple times in the list, the last
 one wins.
 -/
-def materializeUpdates (n : Nat) (updates : List (Nat × ValidPos s)) : Vector (ValidPosPlusOne s) n :=
+def materializeUpdates (n : Nat) (updates : List (Nat × Pos s)) : Vector (ValidPosPlusOne s) n :=
   materializeUpdatesAux n (Vector.replicate n (.sentinel s)) updates
 
-def equivPos {s} (p : Option (ValidPos s)) (p' : ValidPosPlusOne s) : Prop :=
+def equivPos {s} (p : Option (Pos s)) (p' : ValidPosPlusOne s) : Prop :=
   match p with
   | .some p => p' = .validPos p
   | .none => p' = .sentinel s
 
 @[simp, grind =]
-theorem equivPos.some_iff {p : ValidPos s} {p' : ValidPosPlusOne s} : equivPos (.some p) p' ↔ p' = .validPos p := by
+theorem equivPos.some_iff {p : Pos s} {p' : ValidPosPlusOne s} : equivPos (.some p) p' ↔ p' = .validPos p := by
   grind [equivPos]
 
 @[simp, grind =]
@@ -51,7 +51,7 @@ theorem equivPos.none_iff {p' : ValidPosPlusOne s} : equivPos .none p' ↔ p' = 
   grind [equivPos]
 
 @[simp, grind =]
-theorem equivPos.validPos_iff {p p' : ValidPos s} : equivPos p (.validPos p') ↔ p = p' := by
+theorem equivPos.validPos_iff {p p' : Pos s} : equivPos p (.validPos p') ↔ p = p' := by
   grind [equivPos]
 
 @[simp, grind =]
@@ -60,13 +60,13 @@ theorem equivPos.sentinel_iff {p} : equivPos p (.sentinel s) ↔ p = .none := by
   | .some p => simpa using ValidPosPlusOne.validPos_ne_sentinel.symm
   | .none => simp
 
-def EquivMaterializedUpdate {n} (groups : Nat → Option (ValidPos s × ValidPos s)) (updates : Vector (ValidPosPlusOne s) n) : Prop :=
+def EquivMaterializedUpdate {n} (groups : Nat → Option (Pos s × Pos s)) (updates : Vector (ValidPosPlusOne s) n) : Prop :=
   ∀ tag,
     ((h₁ : 2 * tag < n) → (equivPos ((groups tag).map (·.1)) updates[2 * tag])) ∧
     ((h₂ : 2 * tag + 1 < n) → (equivPos ((groups tag).map (·.2)) updates[2 * tag + 1]))
 
-theorem EquivMaterializedUpdate.eq {n} {groups : Nat → Option (ValidPos s × ValidPos s)} {updates : Vector (ValidPosPlusOne s) n}
-  (eqv : EquivMaterializedUpdate groups updates) (tag : Nat) (lt : 2 * tag + 1 < n) (p₁ p₂ : ValidPos s) :
+theorem EquivMaterializedUpdate.eq {n} {groups : Nat → Option (Pos s × Pos s)} {updates : Vector (ValidPosPlusOne s) n}
+  (eqv : EquivMaterializedUpdate groups updates) (tag : Nat) (lt : 2 * tag + 1 < n) (p₁ p₂ : Pos s) :
   groups tag = .some (p₁, p₂) ↔ updates[2 * tag] = .validPos p₁ ∧ updates[2 * tag + 1] = .validPos p₂ := by
   have eq₁ := (eqv tag).1 (by grind)
   have eq₂ := (eqv tag).2 lt
@@ -74,8 +74,8 @@ theorem EquivMaterializedUpdate.eq {n} {groups : Nat → Option (ValidPos s × V
   | .some (p₁', p₂') => grind
   | .none => grind
 
-theorem EquivMaterializedUpdate.eq_none {n} {groups : Nat → Option (ValidPos s × ValidPos s)} {updates : Vector (ValidPosPlusOne s) n}
-  (eqv : EquivMaterializedUpdate groups updates) (tag : Nat) (lt : 2 * tag + 1 < n) (p₁ p₂ : ValidPos s) :
+theorem EquivMaterializedUpdate.eq_none {n} {groups : Nat → Option (Pos s × Pos s)} {updates : Vector (ValidPosPlusOne s) n}
+  (eqv : EquivMaterializedUpdate groups updates) (tag : Nat) (lt : 2 * tag + 1 < n) :
   groups tag = .none ↔ updates[2 * tag] = .sentinel s ∧ updates[2 * tag + 1] = .sentinel s := by
   have eq₁ := (eqv tag).1 (by grind)
   have eq₂ := (eqv tag).2 lt
