correctness/RegexCorrectness/VM/EpsilonClosure/Lemmas.lean
@@ -8,13 +8,13 @@ set_option autoImplicit false
 open Regex.Data (SparseSet)
 open Regex (NFA)
 open Regex.NFA (εStep')
-open String (ValidPos)
+open String (Pos)
 
 namespace Regex.VM.εClosure
 
 namespace pushNext
 
-variable {s : String} {σ : Strategy s} {nfa : NFA} {pos : ValidPos s} {node : NFA.Node}
+variable {s : String} {σ : Strategy s} {nfa : NFA} {pos : Pos s} {node : NFA.Node}
   {inBounds : node.inBounds nfa.nodes.size} {update : σ.Update} {stack : εStack σ nfa}
 
 theorem mem_of_mem_stack {entry} (mem : entry ∈ stack) :
@@ -26,7 +26,7 @@ end pushNext
 -- Theorems that hold for any strategy
 section
 
-variable {s : String} {σ : Strategy s} {nfa : NFA} {wf : nfa.WellFormed} {pos : ValidPos s}
+variable {s : String} {σ : Strategy s} {nfa : NFA} {wf : nfa.WellFormed} {pos : Pos s}
   {matched : Option σ.Update} {next : SearchState σ nfa} {stack : εStack σ nfa}
   {matched' : Option σ.Update} {next' : SearchState σ nfa}
 
@@ -171,21 +171,21 @@ theorem not_done_of_none (result) (h : εClosure σ nfa wf pos matched next stac
       | inr mem => exact inv i mem
     exact ih h inv'
 
-def LowerInvStep (pos : ValidPos s) (states : SparseSet nfa.nodes.size) (stack : εStack σ nfa) : Prop :=
+def LowerInvStep (pos : Pos s) (states : SparseSet nfa.nodes.size) (stack : εStack σ nfa) : Prop :=
   ∀ i j update, i ∈ states → nfa.εStep' pos i j update → j ∈ states ∨ ∃ update', (update', j) ∈ stack
 
-def LowerBoundStep (pos : ValidPos s) (states : SparseSet nfa.nodes.size) : Prop :=
+def LowerBoundStep (pos : Pos s) (states : SparseSet nfa.nodes.size) : Prop :=
   ∀ i j update, i ∈ states → nfa.εStep' pos i j update → j ∈ states
 
-def LowerBound (pos : ValidPos s) (states : SparseSet nfa.nodes.size) : Prop :=
+def LowerBound (pos : Pos s) (states : SparseSet nfa.nodes.size) : Prop :=
   ∀ i j update, i ∈ states → nfa.εClosure' pos i j update → j ∈ states
 
-theorem LowerBound.of_empty {pos : ValidPos s} {states : SparseSet nfa.nodes.size} (h : states.isEmpty) :
+theorem LowerBound.of_empty {pos : Pos s} {states : SparseSet nfa.nodes.size} (h : states.isEmpty) :
   LowerBound pos states := by
   intro i j update mem cls
   exact (SparseSet.not_mem_of_isEmpty h mem).elim
 
-theorem LowerBound.of_step {pos : ValidPos s} {states : SparseSet nfa.nodes.size} (h : LowerBoundStep pos states) :
+theorem LowerBound.of_step {pos : Pos s} {states : SparseSet nfa.nodes.size} (h : LowerBoundStep pos states) :
   εClosure.LowerBound pos states := by
   intro i j update mem cls
   induction cls with
@@ -282,7 +282,7 @@ theorem preserves (wf : nfa.WellFormed) (hmem : entry.2 ∉ states) (inv : Lower
 
 end LowerInvStep
 
-theorem lower_bound_step {pos : ValidPos s} (h : εClosure σ nfa wf pos matched next stack = (matched', next'))
+theorem lower_bound_step {pos : Pos s} (h : εClosure σ nfa wf pos matched next stack = (matched', next'))
   (inv : LowerInvStep pos next.states stack) :
   LowerBoundStep pos next'.states := by
   induction matched, next, stack using εClosure.induct' σ nfa wf pos with
@@ -321,9 +321,9 @@ end
 -- Theorems that hold for HistoryStrategy
 section
 
-variable {s : String} {nfa : NFA} {wf : nfa.WellFormed} {pos : ValidPos s}
-  {matched : Option (List (Nat × ValidPos s))} {next : SearchState (HistoryStrategy s) nfa} {stack : εStack (HistoryStrategy s) nfa}
-  {matched' : Option (List (Nat × ValidPos s))} {next' : SearchState (HistoryStrategy s) nfa}
+variable {s : String} {nfa : NFA} {wf : nfa.WellFormed} {pos : Pos s}
+  {matched : Option (List (Nat × Pos s))} {next : SearchState (HistoryStrategy s) nfa} {stack : εStack (HistoryStrategy s) nfa}
+  {matched' : Option (List (Nat × Pos s))} {next' : SearchState (HistoryStrategy s) nfa}
 
 /--
 Intuition: given that we reached `i₀` (from `nfa.start`) with `pos₀` and `update₀`, the εClosure
@@ -335,7 +335,7 @@ doesn't change during the traversal.
 At the end of the traversal, we can guarantee that all states in `next` were already in `states₀` or
 they are reachable from `i₀` with the updates written to `next.updates`.
 -/
-structure UpperInv (states₀ : SparseSet nfa.nodes.size) (pos₀ : ValidPos s) (i₀ : Fin nfa.nodes.size) (update₀ : List (Nat × ValidPos s))
+structure UpperInv (states₀ : SparseSet nfa.nodes.size) (pos₀ : Pos s) (i₀ : Fin nfa.nodes.size) (update₀ : List (Nat × Pos s))
   (next : SearchState (HistoryStrategy s) nfa) (stack : εStack (HistoryStrategy s) nfa) : Prop where
   -- The intuition is that `update₀` corresponds to the update list from `nfa.start` to `i₀`, and
   -- `update'` is the update list from `i₀` to `j`. Therefore, `update₀ ++ update'` gives the update
@@ -347,8 +347,8 @@ structure UpperInv (states₀ : SparseSet nfa.nodes.size) (pos₀ : ValidPos s) 
 
 namespace UpperInv
 
-variable {states₀ : SparseSet nfa.nodes.size} {pos₀ : ValidPos s} {i₀ : Fin nfa.nodes.size} {update₀ : List (Nat × ValidPos s)}
-  {next : SearchState (HistoryStrategy s) nfa} {entry : List (Nat × ValidPos s) × Fin nfa.nodes.size} {stack : εStack (HistoryStrategy s) nfa}
+variable {states₀ : SparseSet nfa.nodes.size} {pos₀ : Pos s} {i₀ : Fin nfa.nodes.size} {update₀ : List (Nat × Pos s)}
+  {next : SearchState (HistoryStrategy s) nfa} {entry : List (Nat × Pos s) × Fin nfa.nodes.size} {stack : εStack (HistoryStrategy s) nfa}
 
 theorem preserves' {stack'} {node} (hn : nfa[entry.2] = node) (nextEntries) (hstack : stack' = nextEntries ++ stack)
   (not_mem : entry.2 ∉ next.states)
@@ -390,7 +390,7 @@ theorem preserves' {stack'} {node} (hn : nfa[entry.2] = node) (nextEntries) (hst
           exact h write
         next => exact h write
 
-theorem preserves {update : List (Nat × ValidPos s)} {state : Fin nfa.nodes.size} (wf : nfa.WellFormed) (not_mem : state ∉ next.states)
+theorem preserves {update : List (Nat × Pos s)} {state : Fin nfa.nodes.size} (wf : nfa.WellFormed) (not_mem : state ∉ next.states)
   (inv : UpperInv states₀ pos₀ i₀ update₀ next ((update, state) :: stack)) :
   letI states' := next.states.insert state not_mem
   letI updates' := if writeUpdate nfa[state] then next.updates.set state update else next.updates
@@ -436,7 +436,7 @@ end UpperInv
 /--
 All new states in `next'` are reachable from the starting state `i₀` and have corresponding updates in `next'.updates`.
 -/
-theorem upper_boundAux (states₀ : SparseSet nfa.nodes.size) (pos₀ : ValidPos s) (i₀ : Fin nfa.nodes.size) (update₀ : List (Nat × ValidPos s))
+theorem upper_boundAux (states₀ : SparseSet nfa.nodes.size) (pos₀ : Pos s) (i₀ : Fin nfa.nodes.size) (update₀ : List (Nat × Pos s))
   (h : εClosure (HistoryStrategy s) nfa wf pos₀ matched next stack = (matched', next'))
   (inv₀ : UpperInv states₀ pos₀ i₀ update₀ next stack) :
   UpperInv states₀ pos₀ i₀ update₀ next' []  := by
@@ -464,7 +464,7 @@ theorem upper_boundAux (states₀ : SparseSet nfa.nodes.size) (pos₀ : ValidPos
 /--
 Upper invariant at the start of the εClosure traversal.
 -/
-theorem UpperInv.intro {i₀ update₀} (pos₀ : ValidPos s) :
+theorem UpperInv.intro {i₀ update₀} (pos₀ : Pos s) :
   εClosure.UpperInv next.states pos₀ i₀ update₀ next [(update₀, i₀)] := by
   refine ⟨?mem_stack, ?mem_next⟩
   case mem_stack =>
@@ -474,7 +474,7 @@ theorem UpperInv.intro {i₀ update₀} (pos₀ : ValidPos s) :
     intro j mem
     exact .inl mem
 
-theorem upper_bound {i} {update : List (Nat × ValidPos s)}
+theorem upper_bound {i} {update : List (Nat × Pos s)}
   (h : εClosure (HistoryStrategy s) nfa wf pos matched next [(update, i)] = (matched', next')) :
   ∀ j ∈ next'.states, j ∈ next.states ∨
     ∃ update', nfa.εClosure' pos i j update' ∧ (writeUpdate nfa[j] → next'.updates[j] = update ++ update') := by
@@ -496,7 +496,7 @@ theorem mem_next {i update}
 All states in `next'.states` are already in `next.states` or they are reachable from `i` with the
 updates written to `next'.updates`.
 -/
-theorem write_updates_of_mem_next {i j} {update : List (Nat × ValidPos s)}
+theorem write_updates_of_mem_next {i j} {update : List (Nat × Pos s)}
   (h : εClosure (HistoryStrategy s) nfa wf pos matched next [(update, i)] = (matched', next')) (mem : j ∈ next'.states) :
   j ∈ next.states ∨ ∃ update', nfa.εClosure' pos i j update' ∧ (writeUpdate nfa[j] → next'.updates[j] = update ++ update') :=
   εClosure.upper_bound h j mem
@@ -506,7 +506,7 @@ For all states in the ε-closure of `i`, it's already in `next.states` or there 
 whose updates are written to `next.updates`. The written update list can be different since the
 traversal may have reached the state through a different path.
 -/
-theorem write_updates {i j} {update update' : List (Nat × ValidPos s)}
+theorem write_updates {i j} {update update' : List (Nat × Pos s)}
   (h : εClosure (HistoryStrategy s) nfa wf pos matched next [(update, i)] = (matched', next'))
   (lb : εClosure.LowerBound pos next.states) (cls : nfa.εClosure' pos i j update') :
   j ∈ next.states ∨ ∃ update', nfa.εClosure' pos i j update' ∧ (writeUpdate nfa[j] → next'.updates[j] = update ++ update') :=
