correctness/RegexCorrectness/Backtracker/Compile.lean
@@ -4,7 +4,7 @@ import RegexCorrectness.NFA.Semantics
 
 set_option autoImplicit false
 
-open String (ValidPos)
+open String (Pos)
 open Regex.NFA (EquivUpdate)
 open Regex.Data (CaptureGroups BitMatrix BVPos)
 
@@ -14,7 +14,7 @@ namespace captureNext
 
 theorem path_done_of_some {s nfa wf pos update} (hres : captureNext (HistoryStrategy s) nfa wf pos = .some update) :
   ∃ state pos' pos'', nfa[state] = .done ∧ pos ≤ pos' ∧ Path nfa wf pos' pos'' state update := by
-  let bvpos : BVPos pos := ⟨pos, ValidPos.le_refl _⟩
+  let bvpos : BVPos pos := ⟨pos, Pos.le_refl _⟩
   dsimp [captureNext] at hres
   have ⟨state, bvpos', bvpos'', hn, le, path⟩ := go.path_done_of_some hres
   exact ⟨state, bvpos'.current, bvpos''.current, hn, le, path⟩
@@ -32,25 +32,25 @@ theorem capture_of_some_compile {s e pos update} (hres : captureNext (HistoryStr
   exact ⟨pos', pos'', groups, le, c, eqv⟩
 
 theorem ne_done_of_path_of_none {s nfa wf pos} (hres : captureNext (HistoryStrategy s) nfa wf pos = .none) :
-  ∀ (pos' pos'' : ValidPos s) (state : Fin nfa.nodes.size) (update : List (Nat × ValidPos s)),
+  ∀ (pos' pos'' : Pos s) (state : Fin nfa.nodes.size) (update : List (Nat × Pos s)),
     pos ≤ pos' →
     Path nfa wf pos' pos'' state update →
     nfa[state] ≠ .done := by
   dsimp [captureNext] at hres
 
-  let bvpos : BVPos pos := ⟨pos, ValidPos.le_refl _⟩
+  let bvpos : BVPos pos := ⟨pos, Pos.le_refl _⟩
   let visited := BitMatrix.zero nfa.nodes.size (pos.remainingBytes + 1)
 
   have h := go.ne_done_of_path_of_none hres (BVPos.le_refl _) go.Inv.zero captureNextAux.NotDoneInv.zero
 
   intro pos' pos'' state update le path hn
   let bvpos' : BVPos pos := ⟨pos', le⟩
-  let bvpos'' : BVPos pos := ⟨pos'', ValidPos.le_trans le path.le⟩
+  let bvpos'' : BVPos pos := ⟨pos'', Pos.le_trans le path.le⟩
 
   exact h bvpos' bvpos'' state update bvpos'.le path hn
 
 theorem not_captures_of_none_compile {s e pos} (hres : captureNext (HistoryStrategy s) (NFA.compile e) NFA.compile_wf pos = .none)
-  (pos' pos'' : ValidPos s) (groups : CaptureGroups s) (le : pos ≤ pos') :
+  (pos' pos'' : Pos s) (groups : CaptureGroups s) (le : pos ≤ pos') :
   ¬e.Captures pos' pos'' groups := by
   intro c
   have ⟨update, _, path⟩ := NFA.path_of_captures_compile rfl c
