correctness/RegexCorrectness/Backtracker/Correctness.lean
@@ -8,14 +8,14 @@ open Regex (NFA)
 open Regex.Data (Expr CaptureGroups)
 open Regex.Strategy (EquivMaterializedUpdate materializeRegexGroups materializeUpdates)
 open RegexCorrectness.Spec (SearchProblem)
-open String (ValidPos)
+open String (Pos)
 
 namespace Regex.Backtracker
 
 theorem captureNext_soundness {s e bufferSize pos matchedB}
   (disj : e.Disjoint)
   (hresB : captureNext (BufferStrategy s bufferSize) (NFA.compile e) NFA.compile_wf pos = .some matchedB) :
-  ∃ (pos' pos'' : ValidPos s) (groups : CaptureGroups s),
+  ∃ (pos' pos'' : Pos s) (groups : CaptureGroups s),
     pos ≤ pos' ∧
     e.Captures pos' pos'' groups ∧
     EquivMaterializedUpdate (materializeRegexGroups groups) matchedB := by
@@ -31,7 +31,7 @@ theorem captureNext_soundness {s e bufferSize pos matchedB}
 
 theorem captureNext_completeness' {s e bufferSize pos}
   (hresB : captureNext (BufferStrategy s bufferSize) (NFA.compile e) NFA.compile_wf pos = .none)
-  (pos' pos'' : ValidPos s) (groups : CaptureGroups s) (le : pos ≤ pos') (c : e.Captures pos' pos'' groups) :
+  (pos' pos'' : Pos s) (groups : CaptureGroups s) (le : pos ≤ pos') (c : e.Captures pos' pos'' groups) :
   False := by
   match hresH : captureNext (HistoryStrategy s) (NFA.compile e) NFA.compile_wf pos with
   | .some matchedH =>
@@ -41,13 +41,13 @@ theorem captureNext_completeness' {s e bufferSize pos}
 
 theorem captureNext_completeness {s e bufferSize pos}
   (hresB : captureNext (BufferStrategy s bufferSize) (NFA.compile e) NFA.compile_wf pos = .none) :
-  ¬∃ (pos' pos'' : ValidPos s) (groups : CaptureGroups s),
+  ¬∃ (pos' pos'' : Pos s) (groups : CaptureGroups s),
     pos ≤ pos' ∧
     e.Captures pos' pos'' groups := by
   grind [captureNext_completeness']
 
 -- NOTE: we don't make this an instance because there are multiple decision procedures
-def decideSearchProblem {s : String} (e : Expr) (pos : ValidPos s) (disj : e.Disjoint) : Decidable (SearchProblem e pos) :=
+def decideSearchProblem {s : String} (e : Expr) (pos : Pos s) (disj : e.Disjoint) : Decidable (SearchProblem e pos) :=
   match hresB : captureNext (BufferStrategy s 0) (NFA.compile e) NFA.compile_wf pos with
   | .some _ => .isTrue <|
     have ⟨pos', pos'', groups, le, c, _⟩ := captureNext_soundness disj hresB
